Eff.fst
@@ -121,7 +121,7 @@ let perform #ops #eqs (op:op{op `mem` ops}) (x:param_of op)
 
 (* Effect handlers (on Eff effect representations) *)
 
-let raw_eff_handler (ops:sig) (eqs:equations ops) (a:Type) (ops':sig) (eqs':equations ops') 
+let eff_handler_raw (ops:sig) (eqs:equations ops) (a:Type) (ops':sig) (eqs':equations ops') 
   = op:op{op `mem` ops} -> param_of op -> (arity_of op -> eff a ops' eqs') -> eff a ops' eqs'
 
 let rec to_respects_hypotheses a #ops (eqs:equations ops) 
@@ -133,40 +133,52 @@ let rec to_respects_hypotheses a #ops (eqs:equations ops)
       /\
       to_respects_hypotheses a eqs'
 
-(*
-let rec to_respects_conclusion #a #ops #ops' (eqs:equations ops) #eqs' (h:raw_eff_handler ops eqs a ops' eqs')
-  : Type0
-  = match eqs with
-    | [] -> unit
-    | eq :: eqs'' -> 
-        squash(eq_to_prop (to_inst_equation eq h))
-        *
-        to_respects_conclusion eqs'' h
-*)
-
-let rec to_respects_conclusion #a #ops #ops' (eqs:equations ops) #eqs' (h:raw_eff_handler ops eqs a ops' eqs')
-  : Type0
-  = match eqs with
-    | [] -> unit
-    | eq :: eqs'' -> 
-        eq_to_prop (to_inst_equation eq (T.id_template_handler a ops))
-        /\
-        to_respects_conclusion eqs'' h
-
 let eff_norm_steps = [delta;zeta;primops;simplify;iota]
 
-let eff_handler_respects (ops:sig) (eqs:equations ops) (a:Type) (ops':sig) (eqs':equations ops') (h:raw_eff_handler ops eqs a ops' eqs') =
-  unit -> Pure unit
+let rec eff_handler_respects (ops:sig) (eqs:equations ops) (a:Type) (ops':sig) (eqs':equations ops') (h:eff_handler_raw ops eqs a ops' eqs') =
+  match eqs with
+  | [] -> unit
+  | eq :: eqs'' -> 
+      (unit -> Pure unit
               (requires (norm eff_norm_steps (to_respects_hypotheses a eqs')))
-              (ensures  (fun _ -> norm eff_norm_steps (to_respects_conclusion eqs h)))
+              (ensures  (fun _ -> norm eff_norm_steps (eq_to_prop (to_inst_equation eq h)))))
+      *
+      eff_handler_respects ops eqs'' a ops' eqs' h
 
 let eff_handler (ops:sig) (eqs:equations ops) (a:Type) (ops':sig) (eqs':equations ops')
-  = h:raw_eff_handler ops eqs a ops' eqs'
+  = h:eff_handler_raw ops eqs a ops' eqs'
     & 
     eff_handler_respects ops eqs a ops' eqs' h
 
-let eff_respects = fun () -> ()
 
+(* Effect handlers (on the Eff effect) *)
+
+let handler_raw (ops:sig) (eqs:equations ops) (a:Type) (ops':sig) (eqs':equations ops') 
+  = op:op{op `mem` ops} -> param_of op -> (arity_of op -> Eff a ops' eqs') -> Eff a ops' eqs'
+
+let reflect_cont #a #b #ops #eqs (k:b -> eff a ops eqs) (y:b) : Eff a ops eqs
+  = Eff?.reflect (k y)
+
+let to_eff_handler #ops #eqs #a #ops' #eqs'
+  (h:handler_raw ops eqs a ops' eqs')
+  : eff_handler_raw ops eqs a ops' eqs'
+  = fun op x k ->  
+      (reify (h op x (reflect_cont k))) 
+
+let rec handler_respects (ops:sig) (eqs:equations ops) (a:Type) (ops':sig) (eqs':equations ops') (h:handler_raw ops eqs a ops' eqs') =
+  match eqs with
+  | [] -> unit
+  | eq :: eqs'' -> 
+      (unit -> Pure unit
+              (requires (norm eff_norm_steps (to_respects_hypotheses a eqs')))
+              (ensures  (fun _ -> norm eff_norm_steps (eq_to_prop (to_inst_equation eq (to_eff_handler h))))))
+      *
+      handler_respects ops eqs'' a ops' eqs' h
+
+let handler (ops:sig) (eqs:equations ops) (a:Type) (ops':sig) (eqs':equations ops')
+  = h:handler_raw ops eqs a ops' eqs'
+    & 
+    handler_respects ops eqs a ops' eqs' h
 
 
 
